examples/opaque: begin work on game proof

examples/opaque/server_proofs.v
@@ -21,13 +21,13 @@ Context `{!cryptisGS Σ, !heapGS Σ, !spawnG Σ}.
 
 Notation iProp := (iProp Σ).
 
-Definition opaque_file (file : term) : iProp :=
+Definition opaque_file (file : val) : iProp :=
   ∃ k_s p_s P_s P_u envelope,
     ⌜file = Spec.of_list [k_s; p_s; P_s; P_u; envelope]⌝
     ∗ minted k_s ∗ minted p_s ∗ public P_s ∗ public P_u ∗ public envelope.
 
-Definition opaque_db (db : gmap term term) : iProp :=
-[∗ map] (k : term) ↦ (file : term) ∈ db,
+Definition opaque_db (db : gmap term val) : iProp :=
+[∗ map] (k : term) ↦ (file : val) ∈ db,
 public k ∗ opaque_file file.
 
 Lemma public_THashE N φ t :
@@ -111,43 +111,44 @@ Proof.
     do !iSplit => //; do ?iApply public_TExp => //; by rewrite public_TInt.
 Qed.
 
-Lemma wp_server_session (db c : term) (alist : gmap term term) :
-cryptis_ctx -∗
-hash_pred (opN.@"A_s") (λ _,  True) -∗
-channel c -∗
-AList.is_alist db (repr <$> alist) -∗
-opaque_db alist -∗
-WP Server.session db c
-{{ x , True }}.
+Lemma wp_server_session (db c : val) (alist : gmap term val) :
+{{{ cryptis_ctx
+      ∗ hash_pred (opN.@"A_s") (λ _,  True)
+      ∗ channel c
+      ∗ AList.is_alist db alist
+      ∗ opaque_db alist }}}
+  Server.session db c
+{{{ x , RET x ; True }}}.
 Proof.
+  iIntros "%ϕ".
   rewrite /opaque_db big_sepM_forall.
-  iIntros "#Cryptis #Hpred #Hc Hdb #Hmapcontents".
+  iIntros "[#Cryptis [#Hpred [#Hc [Hdb #Hmapcontents]]]] Hhl".
   wp_lam. wp_pures.
   wp_apply (wp_recv with "Hc").
   iIntros "%m1 #Hpubm1".
   wp_list_of_term m1; wp_pures.
-  2: by iModIntro.
+  2: iModIntro; by iApply "Hhl".
   do !rewrite subst_list_match /=.
   wp_list_match => [uid α X_u | _].
-  2: wp_pures; by iModIntro.
+  2: wp_pures; iModIntro; by iApply "Hhl".
   intro Hm1eq.
   wp_bind (AList.find _ _).
   iApply (AList.wp_find with "Hdb").
-  iIntros "!> Hdb". rewrite lookup_fmap.
+  iIntros "!> Hdb".
   case db_uid: (alist !! uid) => [file|]; wp_pures.
-  2: by iModIntro.
+  2: iModIntro; by iApply "Hhl".
   iDestruct ("Hmapcontents" $! uid file with "[//]") as
   "[_ (%k_s & %p_s & %P_s & %P_u & %envelope &
         %e & Hmk_s & Hmp_s & HpP_s & HpP_u & Hpenvelope)]".
   repeat rewrite subst_list_match /=.
-  wp_apply wp_list_of_term.
   rewrite e.
+  wp_apply wp_list_of_term.
   rewrite Spec.of_listK.
   wp_pures.
   rewrite subst_list_match /=.
   wp_list_match => [k_s' p_s' P_s' P_u' envelope' e' | ].
   inversion e'. subst. clear e'.
-  2: intro H; wp_pures; by iModIntro.
+  2: intro H; wp_pures; iModIntro; by iApply "Hhl".
   wp_apply (wp_mk_nonce (fun _ => False)%I (fun _ => True)%I).
   1: iAssumption.
   iIntros "%x_s %Hnoncex_s #Hmintedx_s #Hprivatex_s #Hdhx_s Htokenx_s".
@@ -167,8 +168,7 @@ Proof.
   wp_list.
   wp_term_of_list.
   wp_pures.
-  rewrite public_of_list.
-  simpl.
+  rewrite public_of_list => /=.
   iDestruct "Hpubm1" as "[Hpubuid [Hpubα [HpubX_u _]]]".
   wp_apply wp_send => //.
   1: rewrite public_of_list => //.
@@ -194,10 +194,11 @@ Proof.
   wp_list.
   wp_apply wp_prf.
   wp_eq_term Heq; wp_pures.
-  2: by iModIntro.
+  2: iModIntro; by iApply "Hhl".
   wp_list.
   wp_pures.
-  by iModIntro.
+  iModIntro.
+  by iApply "Hhl".
 Admitted.
 
 End Opaque.
