examples/opaque/game.v
@@ -11,8 +11,8 @@ From iris.heap_lang Require Import notation proofmode.
 From iris.heap_lang.lib Require Import lock ticket_lock.
 From cryptis.examples Require Import alist.
 
-From cryptis.examples.opaque Require Import impl.
-From cryptis Require Import primitives.
+From cryptis.examples.opaque Require Import impl server_proofs client_proofs.
+From cryptis Require Import lib term cryptis primitives tactics.
 
 Set Implicit Arguments.
 Unset Strict Implicit.
@@ -20,7 +20,7 @@ Unset Printing Implicit Defensive.
 
 Section Game.
 
-Context `{!cryptisGS Σ, !heapGS Σ, !spawnG Σ, !sessionGS Σ, !metaGS Σ}.
+Context `{!cryptisGS Σ, !heapGS Σ, !spawnG Σ}.
 Notation iProp := (iProp Σ).
 
 Notation opN := (nroot.@"op").
@@ -35,5 +35,68 @@ AList.insert "db" "uid" (Server.make_file "pw") ;;
 Fork (Server.session "db" "c");;
 Client.session "uid" "c" "pw";;
 assert: (~ eq_term "pw" (recv "c")).
+
+Lemma wp_game :
+{{{ cryptis_ctx }}}
+game #()
+{{{ x , RET x ; True }}}.
+Proof.
+iIntros "%ϕ #Hcryptis Hhl".
+wp_lam.
+wp_apply wp_init_network => //.
+iIntros "%c #Hchannel".
+wp_pures.
+wp_apply (wp_mk_nonce (fun _ => True)%I (fun _ => False)%I) => //.
+iIntros "%uid %Hnonceuid #Hminuid #Hpubuid #Hdhuid Htermtokenuid".
+iDestruct "Hpubuid" as "[_ Hpubuid']".
+iAssert (public uid) as "Hpubuid".
+iApply "Hpubuid'".
+iNext.
+by iModIntro.
+iClear "Hpubuid'".
+wp_pures.
+wp_apply (wp_mk_nonce (fun _ => False)%I (fun _ => False)%I) => //.
+iIntros "%pw %Hnoncepw #Hminpw #Hprivpw #Hdhpw Htermtokenpw".
+wp_pures.
+wp_bind (AList.new #()).
+iApply AList.wp_empty => //.
+iNext.
+iIntros "%db Halist".
+wp_pures.
+wp_apply (wp_make_file pw).
+do !iSplit => //.
+admit.
+admit.
+admit.
+iIntros "%file Hopaquefile" => /=.
+wp_bind (AList.insert db uid file).
+iApply (AList.wp_insert with "Halist").
+iNext.
+iIntros "Halist".
+wp_pures.
+wp_apply (wp_fork with "[Halist]").
+iApply (wp_server_session db c (<[uid:=file]> ∅)  with "[Halist]") => //.
+do !iSplit => //.
+admit.
+unfold opaque_db.
+admit.
+wp_pures.
+wp_bind (Client.session uid c pw).
+iApply (wp_client_session uid pw c).
+do !iSplit => //.
+admit.
+iNext.
+iIntros "%_ _".
+wp_pures.
+wp_apply wp_assert.
+wp_apply wp_recv => //.
+iIntros "%attack #Hpubattack".
+wp_eq_term H; wp_pures; iModIntro; iSplit => //.
+2, 3: by iApply "Hhl".
+rewrite H.
+iDestruct "Hprivpw" as "[Hprivpw _]".
+iDestruct ("Hprivpw" with "Hpubattack") as "Hcontra".
+iPureIntro.
+Admitted.
 
 End Game.
